Finished the lifting safety.

concurrency/lifting_safety.v
@@ -25,6 +25,7 @@ Require Import concurrency.machine_simulation. Import machine_simulation.
 
 Require Import concurrency.HybridMachine_simulation_proof.
 
+Set Bullet Behavior "Strict Subproofs".
 
 Module lifting_safety.
   Import DMS.
@@ -45,23 +46,22 @@ Module lifting_safety.
          (ptgt : option DryMachine.ThreadPool.RES.res) (sch : SC.Sch).
   Definition the_simulation:=
     lifting.concur_sim p tp compiled
-                       Values.Vundef psrc ptgt sch.
+                       psrc ptgt sch.
   
   
   Lemma safety_preservation'':
-        forall Sg Tg tr Sds Sm Tds Tm cd
+        forall  tr Sds Sm Tds Tm cd
           (MATCH: exists j, (MSmatch_states Values.Vundef the_simulation) cd j Sds Sm Tds Tm),
           (forall sch, DMS.DryConc.new_valid (tr, Sds, Sm) sch ->
-                  DMS.DryConc.explicit_safety Sg sch Sds Sm) ->
+                  DMS.DryConc.explicit_safety (fst genv') sch Sds Sm) ->
           (forall sch, DryConc.valid (sch, tr, Tds) ->
                   DryConc.stutter_stepN_safety
-                    (core_ord:=MSorder Values.Vundef the_simulation) Tg cd sch Tds Tm).
+                    (core_ord:=MSorder Values.Vundef the_simulation) (snd genv') cd sch Tds Tm).
   Proof.
-    move => main psrc ptgt U Sg Tg.
     cofix CIH.
     intros.
     assert (H':=H).
-    specialize (H sch).
+    specialize (H sch0).
     move: MATCH => [] j MATCH.
     assert (equivalid:
                forall cd j Sm Tm tr Sds Tds,
@@ -78,59 +78,42 @@ Module lifting_safety.
               /DryConc.unique_Krun
               /mySchedule.schedPeek /=.
 
-      move => ? ? ? ? ? Sds' Tds' MATCH' sch.
+      move => ? ? ? ? tr0 Sds' Tds' MATCH' sch.
       destruct (List.hd_error sch); try solve[split; auto].
       split.
       - move => H1  j0 cntj0 q KRUN not_halted.
-        (*eapply H1.*)
-        (*pose (same_running Tg Sg main p U cd j Sds' Sm Tds' Tm).*)
-        pose ( machine_semantics.runing_thread (new_DMachineSem sch None)).
-        unfold new_DMachineSem  in P; simpl in P.
-        unfold DMS.DryConc.unique_Krun in P.
-        eapply P.
+        eapply the_simulation in KRUN; eauto.
         
-        
-        eapply (same_running) in KRUN; eauto.
       - move => H1  j0 cntj0 q KRUN not_halted.
-
-        (*eapply H1.*)
-        (*pose (same_running Tg Sg main p U cd j Sds' Sm Tds' Tm).*)
-        pose ( machine_semantics.runing_thread (new_DMachineSem sch psrc)).
-        unfold new_DMachineSem  in P; simpl in P.
-        unfold DryConc.unique_Krun in P.
-        eapply (same_running) in KRUN; eauto.
+        eapply the_simulation in KRUN; eauto.
     }
 
     move: (MATCH) => /equivalid /= AA.
-    move: (AA tr sch) => [A B].
-    assert (HH:DryConc.new_valid (tr, Sds, Sm) sch).
-    { (* split.
-      - apply: B. auto.
-      - simpl; assumption. *)
-      apply: B; auto.
+    move: (AA tr sch0) => [A B].
+    assert (HH:DMS.DryConc.new_valid (tr, Sds, Sm) sch0).
+    { apply B; auto.
     }
     apply H in HH.
     move: MATCH.
     inversion HH; clear HH.
     (*Halted case*)
     - {
-      simpl in *; subst.
-      econstructor.
-      move: MATCH H1 => /halt_axiom /= HHH /(halted_trace _ nil nil Sds) AAA.
-      destruct (DryConc.halted (sch, nil ,Sds)) eqn:BBB; try solve [inversion AAA].
-      move: BBB=> /HHH [] j' [] v2 [] inv Halt.
-      rewrite Halt=> //.
+        simpl in *; subst.
+        econstructor.
+        simpl.
+        unfold DMS.DryConc.halted in H1;
+          unfold DryConc.halted; simpl in *.
+        destruct (SCH.schedPeek sch0); eauto.
       Guarded.
       }
 
     - (*Internal StepN case*)
-      { simpl in H2. pose (note2:=5). simpl in *; subst.
-        assert (my_core_diagram:= Machine_sim.thread_diagram
-                           _ _ _ _ _ _ _ _
-                           (concur_sim Tg Sg main psrc ptgt U)).
+      { simpl in H2. simpl in *; subst.
+        assert (my_core_diagram:= MSthread_diagram Values.Vundef the_simulation).
         simpl in my_core_diagram.
         intros MATCH.
-        eapply my_core_diagram (*with (st1':= (Tds))(m1':=Tm)*) in MATCH; eauto.
+        destruct y'.
+        eapply my_core_diagram in MATCH; eauto.
         clear my_core_diagram.
         move: MATCH => [] st2' [] m2' [] cd' [] mu' [] MATCH' [step_plus | [] [] n stepN data_step ].
         (*Internal step Plus*)
@@ -141,13 +124,13 @@ Module lifting_safety.
             Lemma thread_stepN_stepN:
               forall Tg n sch Tds Tm st2' m2' U p,
                machine_semantics_lemmas.thread_stepN
-                (Machine.DryConc.new_MachineSemantics U p) Tg n sch Tds
+                (DryConc.new_MachineSemantics U p) Tg n sch Tds
                 Tm st2' m2' ->
                 coinductive_safety.stepN
-                  SC.Sch (Machine.DryMachine.ThreadPool.t * mem)
-                  (fun (U0 : SC.Sch) (stm stm' : Machine.DryMachine.ThreadPool.t * mem)
+                  SC.Sch (DryMachine.ThreadPool.t * mem)
+                  (fun (U0 : SC.Sch) (stm stm' : DryMachine.ThreadPool.t * mem)
                    =>
-                     @Machine.DryConc.internal_step Tg U0 (fst stm) (snd stm)
+                     @DryConc.internal_step Tg U0 (fst stm) (snd stm)
                                                    (fst stm') (snd stm'))
                   sch (Tds, Tm) (st2', m2') n.
             Proof.
@@ -162,40 +145,43 @@ Module lifting_safety.
 
             eapply thread_stepN_stepN; eauto.
           + simpl. intros.
-            eapply CIH with (Sds:=fst y') (Sm:=snd y'); eauto.
+            eapply CIH with (Sds:=t) (Sm:=m); eauto.
+            Guarded.
+            (*
 (*            * a dmit. (* By steping! *) *)
 (*            * destruct H3; auto. (* By steping! *)*)
-            * intros. destruct y' as [a b]; eapply H2.
+            * 
+
+              intros. destruct y' as [a b]; eapply H2.
               auto.
 (*            * simpl in *.
-              destruct H3; eauto. *)
+              destruct H3; eauto. *)*)
 
         -  (*Maybe stutter.... depends on n*)
           destruct n.
           + (*Stutter case*)
             inversion stepN; subst.
             apply coinductive_safety.stutter with (cd':=cd'); auto.
-            apply CIH with (tr:=tr)(Sds:= (fst y') )(Sm:=(snd y')).
+            apply CIH with (tr:=tr)(Sds:= t )(Sm:=m); eauto.
+            (*
 (*            * a dmit. (*by stepping*) *)
 (*            * auto. *)
             * exists mu'; eassumption.
             * destruct y' as [a b]; apply H2; auto.
-            * assumption.
+            * assumption. *)
           + (*Fake stutter case*)
             apply (coinductive_safety.internal_safetyN_stut) with (cd':= cd')(y':=(st2',m2'))(n:=n).
             * eapply thread_stepN_stepN; eauto.
             *  {simpl. intros.
-                eapply CIH with (Sds:=fst y') (Sm:=snd y'). Guarded.
+                eapply CIH with (Sds:=t) (Sm:=m). Guarded.
                 - exists mu'; assumption.
-                - destruct y' as [a b]; eapply H2.
+                - eapply H2.
                - assumption.
  }
       }
-    - (*External step case *)
-      assert (my_machine_diagram:= Machine_sim.machine_diagram
-                           _ _ _ _ _ _ _ _
-                           (concur_sim Tg Sg main psrc ptgt U)).
-        simpl in my_machine_diagram.
+    - 
+      assert (my_machine_diagram:= MSmachine_diagram Values.Vundef the_simulation).
+      simpl in my_machine_diagram.
         intros MATCH.
         eapply my_machine_diagram with (st1':= fst y')(m1':=snd y') in MATCH; eauto.
         + clear my_machine_diagram.
@@ -208,39 +194,41 @@ Module lifting_safety.
             -- assumption.
                Guarded.
 
-               Unshelve.
-               auto.
   Qed.
 
-  Lemma safety_preservation': forall main psrc ptgt U Sg Tg tr Sds Sm Tds Tm
-                                (MATCH: exists cd j, (match_st Tg Sg main psrc ptgt U) cd j Sds Sm Tds Tm),
-      (forall sch, DryConc.valid (sch, tr, Sds) ->
-              DryConc.explicit_safety Sg sch Sds Sm) ->
-      (forall sch, Machine.DryConc.valid (sch, tr, Tds) ->
-              Machine.DryConc.explicit_safety Tg sch Tds Tm).
+
+  
+    Lemma safety_preservation':
+      forall tr Sds Sm Tds Tm cd
+        (MATCH: exists j, (MSmatch_states Values.Vundef the_simulation) cd j Sds Sm Tds Tm),
+      (forall sch, DMS.DryConc.valid (sch, tr, Sds) ->
+              DMS.DryConc.explicit_safety (fst genv') sch Sds Sm) ->
+      (forall sch, DryConc.valid (sch, tr, Tds) ->
+              DryConc.explicit_safety (snd genv') sch Tds Tm).
   Proof.
-    move=> main psrc ptgt U Sg Tg tr Sds Sm Tds Tm  [] cd  [] mu MATCH HH sch VAL.
+    move=> tr Sds Sm Tds Tm  cd [] j MATCH HH sch VAL.
     apply @coinductive_safety.safety_stutter_stepN_equiv
-    with (core_ord:=core_ord Tg Sg main psrc ptgt U); auto.
-    + apply (core_ord_wf Tg Sg main psrc ptgt U).
-    (* + split; auto; simpl. *)
+    with (core_ord:=MSorder Values.Vundef the_simulation); auto.
+    + eapply MSord_wf; eauto.
     + exists cd.
-      apply safety_preservation'' with (tr:=tr)(Sds:=Sds)(Sm:=Sm); try exists mu; assumption.
+      apply safety_preservation'' with (tr:=tr)(Sds:=Sds)(Sm:=Sm); try exists j; assumption.
+      
   Qed.
 
-  Lemma safety_preservation: forall main psrc ptgt U Sg Tg Sds Sm Tds Tm
-                               (MATCH: exists cd j, (match_st Tg Sg main psrc ptgt U) cd j Sds Sm Tds Tm),
-      (forall sch, DryConc.valid (sch, nil, Sds) ->
-              DryConc.safe_new_step Sg (sch, nil, Sds) Sm) ->
-      (forall sch, Machine.DryConc.valid (sch, nil, Tds) ->
-              Machine.DryConc.safe_new_step Tg (sch, nil, Tds) Tm).
+  Lemma safety_preservation:
+    forall Sds Sm Tds Tm cd
+      (MATCH: exists j, (MSmatch_states Values.Vundef the_simulation) cd j Sds Sm Tds Tm),
+      (forall sch, DMS.DryConc.valid (sch, nil, Sds) ->
+              DMS.DryConc.safe_new_step (fst genv') (sch, nil, Sds) Sm) ->
+      (forall sch, DryConc.valid (sch, nil, Tds) ->
+              DryConc.safe_new_step (snd genv') (sch, nil, Tds) Tm).
   Proof.
     intros.
-    eapply Machine.DryConc.safety_equivalence2; auto.
+    eapply DryConc.safety_equivalence2; auto.
     intros.
     eapply safety_preservation' with (tr:=nil); eauto.
     intros.
-    eapply DryConc.safety_equivalence2; auto.
+    eapply DMS.DryConc.safety_equivalence2; auto.
   Qed.
 
 End lifting_safety.
